share/steel/examples/pulse/parix/Async.fsti
@@ -6,7 +6,7 @@ val asynch (a:Type0) (post : a -> vprop) : Type0
 
 val async_joinable
   (#a : Type0)
-  (post : a -> vprop)
+  (#post : a -> vprop)
   (h : asynch a post)
   : vprop
 
@@ -15,10 +15,10 @@ val async
   (#pre : vprop)
   (#post : (a -> vprop))
   (f : (unit -> stt a pre post))
-  : stt (asynch a post) pre (fun h -> async_joinable post h)
+  : stt (asynch a post) pre (fun h -> async_joinable h)
 
 val await
   (#a : Type0)
   (#post : (a -> vprop))
   (h : asynch a post)
-  : stt a (async_joinable post h) (fun x -> post x)
+  : stt a (async_joinable h) (fun x -> post x)
